testcases/printtest/exec_IR.ll
@@ -1,25 +1,30 @@
-; ModuleID = '/home/clexma/Desktop/Disk_D/Tools/SESL/SESL/build/b-u4m106z0.bc'
+; ModuleID = '/home/clexma/Desktop/Disk_D/Tools/SESL/SESL/build/b-6p6mw4ok.bc'
 source_filename = "llvm-link"
 target datalayout = "e-m:e-p270:32:32-p271:32:32-p272:64:64-i64:64-f80:128-n8:16:32:64-S128"
 target triple = "x86_64-pc-linux-gnu"
 
+%struct.node = type { i32, i32 }
+
 ; Function Attrs: noinline nounwind uwtable
 define dso_local i32 @main() #0 !dbg !7 {
-  %1 = call noalias i8* @malloc(i64 4) #3, !dbg !11, !verifier.code !12
-  %2 = bitcast i8* %1 to i32*, !dbg !11, !verifier.code !12
-  call void @llvm.dbg.value(metadata i32* %2, metadata !13, metadata !DIExpression()), !dbg !15, !verifier.code !12
-  store i32 0, i32* %2, align 4, !dbg !16, !verifier.code !12
-  %3 = call noalias i8* @malloc(i64 8) #3, !dbg !17, !verifier.code !12
-  %4 = bitcast i8* %3 to i32*, !dbg !17, !verifier.code !12
-  call void @llvm.dbg.value(metadata i32* %4, metadata !13, metadata !DIExpression()), !dbg !15, !verifier.code !12
-  %5 = getelementptr inbounds i32, i32* %4, i64 1, !dbg !18, !verifier.code !12
-  store i32 0, i32* %5, align 4, !dbg !19, !verifier.code !12
-  call void @llvm.dbg.value(metadata i32* null, metadata !13, metadata !DIExpression()), !dbg !15, !verifier.code !12
-  %6 = call i32 @foo(), !dbg !20, !verifier.code !12
-  %7 = call i32 @foo(), !dbg !21, !verifier.code !12
-  %8 = call i32 @foo(), !dbg !22, !verifier.code !12
-  %9 = call i32 @foo(), !dbg !23, !verifier.code !12
-  ret i32 0, !dbg !24, !verifier.code !12
+  %1 = call i32 @foo(), !dbg !11, !verifier.code !12
+  ret i32 0, !dbg !13, !verifier.code !12
+}
+
+; Function Attrs: noinline nounwind uwtable
+define internal i32 @foo() #0 !dbg !14 {
+  %1 = alloca %struct.node, align 4, !verifier.code !12
+  %2 = call noalias i8* @malloc(i64 4) #3, !dbg !15, !verifier.code !12
+  %3 = bitcast i8* %2 to i32*, !dbg !15, !verifier.code !12
+  call void @llvm.dbg.value(metadata i32* %3, metadata !16, metadata !DIExpression()), !dbg !18, !verifier.code !12
+  call void @llvm.dbg.value(metadata i32* null, metadata !16, metadata !DIExpression()), !dbg !18, !verifier.code !12
+  call void @llvm.dbg.declare(metadata %struct.node* %1, metadata !19, metadata !DIExpression()), !dbg !25, !verifier.code !12
+  %4 = getelementptr inbounds %struct.node, %struct.node* %1, i32 0, i32 0, !dbg !26, !verifier.code !12
+  store i32 10, i32* %4, align 4, !dbg !27, !verifier.code !12
+  %5 = getelementptr inbounds %struct.node, %struct.node* %1, i32 0, i32 0, !dbg !28, !verifier.code !12
+  %6 = load i32, i32* %5, align 4, !dbg !28, !verifier.code !12
+  call void @none(i32 %6), !dbg !29, !verifier.code !12
+  ret i32 0, !dbg !30, !verifier.code !12
 }
 
 ; Function Attrs: nounwind readnone speculatable willreturn
@@ -29,14 +34,9 @@ declare void @llvm.dbg.declare(metadata, metadata, metadata) #1
 declare dso_local noalias i8* @malloc(i64) #2
 
 ; Function Attrs: noinline nounwind uwtable
-define internal i32 @foo() #0 !dbg !25 {
-  %1 = call noalias i8* @malloc(i64 4) #3, !dbg !26, !verifier.code !12
-  %2 = bitcast i8* %1 to i32*, !dbg !26, !verifier.code !12
-  call void @llvm.dbg.value(metadata i32* %2, metadata !27, metadata !DIExpression()), !dbg !28, !verifier.code !12
-  store i32 0, i32* %2, align 4, !dbg !29, !verifier.code !12
-  call void @llvm.dbg.value(metadata i32* null, metadata !27, metadata !DIExpression()), !dbg !28, !verifier.code !12
-  %3 = ptrtoint i32* null to i32, !dbg !30, !verifier.code !12
-  ret i32 %3, !dbg !31, !verifier.code !12
+define internal void @none(i32 %0) #0 !dbg !31 {
+  call void @llvm.dbg.value(metadata i32 %0, metadata !34, metadata !DIExpression()), !dbg !35, !verifier.code !12
+  ret void, !dbg !36, !verifier.code !12
 }
 
 ; Function Attrs: nounwind readnone speculatable willreturn
@@ -63,28 +63,33 @@ attributes #3 = { nounwind }
 !4 = !{i32 7, !"Dwarf Version", i32 4}
 !5 = !{i32 2, !"Debug Info Version", i32 3}
 !6 = !{i32 1, !"wchar_size", i32 4}
-!7 = distinct !DISubprogram(name: "main", scope: !1, file: !1, line: 3, type: !8, scopeLine: 3, spFlags: DISPFlagDefinition, unit: !0, retainedNodes: !2)
+!7 = distinct !DISubprogram(name: "main", scope: !1, file: !1, line: 8, type: !8, scopeLine: 8, spFlags: DISPFlagDefinition, unit: !0, retainedNodes: !2)
 !8 = !DISubroutineType(types: !9)
 !9 = !{!10}
 !10 = !DIBasicType(name: "int", size: 32, encoding: DW_ATE_signed)
-!11 = !DILocation(line: 4, column: 14, scope: !7)
+!11 = !DILocation(line: 9, column: 5, scope: !7)
 !12 = !{i1 false}
-!13 = !DILocalVariable(name: "x", scope: !7, file: !1, line: 4, type: !14)
-!14 = !DIDerivedType(tag: DW_TAG_pointer_type, baseType: !10, size: 64)
-!15 = !DILocation(line: 0, scope: !7)
-!16 = !DILocation(line: 5, column: 8, scope: !7)
-!17 = !DILocation(line: 6, column: 9, scope: !7)
-!18 = !DILocation(line: 7, column: 9, scope: !7)
-!19 = !DILocation(line: 7, column: 14, scope: !7)
-!20 = !DILocation(line: 9, column: 5, scope: !7)
-!21 = !DILocation(line: 10, column: 5, scope: !7)
-!22 = !DILocation(line: 11, column: 5, scope: !7)
-!23 = !DILocation(line: 12, column: 5, scope: !7)
-!24 = !DILocation(line: 13, column: 5, scope: !7)
-!25 = distinct !DISubprogram(name: "foo", scope: !1, file: !1, line: 15, type: !8, scopeLine: 15, spFlags: DISPFlagDefinition, unit: !0, retainedNodes: !2)
-!26 = !DILocation(line: 16, column: 14, scope: !25)
-!27 = !DILocalVariable(name: "j", scope: !25, file: !1, line: 16, type: !14)
-!28 = !DILocation(line: 0, scope: !25)
-!29 = !DILocation(line: 17, column: 8, scope: !25)
-!30 = !DILocation(line: 19, column: 12, scope: !25)
-!31 = !DILocation(line: 19, column: 5, scope: !25)
+!13 = !DILocation(line: 10, column: 5, scope: !7)
+!14 = distinct !DISubprogram(name: "foo", scope: !1, file: !1, line: 16, type: !8, scopeLine: 16, spFlags: DISPFlagDefinition, unit: !0, retainedNodes: !2)
+!15 = !DILocation(line: 17, column: 14, scope: !14)
+!16 = !DILocalVariable(name: "j", scope: !14, file: !1, line: 17, type: !17)
+!17 = !DIDerivedType(tag: DW_TAG_pointer_type, baseType: !10, size: 64)
+!18 = !DILocation(line: 0, scope: !14)
+!19 = !DILocalVariable(name: "node", scope: !14, file: !1, line: 19, type: !20)
+!20 = !DIDerivedType(tag: DW_TAG_typedef, name: "node_t", file: !1, line: 6, baseType: !21)
+!21 = distinct !DICompositeType(tag: DW_TAG_structure_type, name: "node", file: !1, line: 3, size: 64, elements: !22)
+!22 = !{!23, !24}
+!23 = !DIDerivedType(tag: DW_TAG_member, name: "a", scope: !21, file: !1, line: 4, baseType: !10, size: 32)
+!24 = !DIDerivedType(tag: DW_TAG_member, name: "b", scope: !21, file: !1, line: 5, baseType: !10, size: 32, offset: 32)
+!25 = !DILocation(line: 19, column: 12, scope: !14)
+!26 = !DILocation(line: 20, column: 10, scope: !14)
+!27 = !DILocation(line: 20, column: 12, scope: !14)
+!28 = !DILocation(line: 21, column: 15, scope: !14)
+!29 = !DILocation(line: 21, column: 5, scope: !14)
+!30 = !DILocation(line: 22, column: 5, scope: !14)
+!31 = distinct !DISubprogram(name: "none", scope: !1, file: !1, line: 12, type: !32, scopeLine: 12, flags: DIFlagPrototyped, spFlags: DISPFlagDefinition, unit: !0, retainedNodes: !2)
+!32 = !DISubroutineType(types: !33)
+!33 = !{null, !10}
+!34 = !DILocalVariable(name: "a", arg: 1, scope: !31, file: !1, line: 12, type: !10)
+!35 = !DILocation(line: 0, scope: !31)
+!36 = !DILocation(line: 14, column: 1, scope: !31)
